compiler/dsl/coq/ReflexQuark.v
@@ -10,6 +10,8 @@ Require Import ReflexVec.
 
 Open Scope string_scope.
 
+Module SystemFeatures <: SystemFeaturesInterface.
+
 Definition NB_MSG : nat := 3.
 
 Definition PAYD : vvdesc NB_MSG := mk_vvdesc
@@ -22,27 +24,9 @@ Notation Input   := (None) (only parsing).
 Notation Display := (Some None) (only parsing).
 Notation Quit    := (Some (Some None)) (only parsing).
 
-Definition KSTD : vdesc := mk_vdesc
-  [ fd_d (* curtab *)
-  ; fd_d (* screen *)
-  ; fd_d (* user-input *)
-  ].
+Inductive COMPT' : Set := Tab | Screen | UserInput.
 
-Notation curtab    := (None) (only parsing).
-Notation screen    := (Some None) (only parsing).
-Notation userinput := (Some (Some None)) (only parsing).
-
-Definition IENVD : vdesc := mk_vdesc
-  [ fd_d (* curtab *)
-  ; fd_d (* screen *)
-  ; fd_d (* userinput *)
-  ].
-
-Notation v_t := (None) (only parsing).
-Notation v_s := (Some None) (only parsing).
-Notation v_u := (Some (Some None)) (only parsing).
-
-Inductive COMPT : Set := Tab | Screen | UserInput.
+Definition COMPT := COMPT'.
 
 Definition COMPTDEC : forall (x y : COMPT), decide (x = y).
 Proof. decide equality. Defined.
@@ -54,70 +38,118 @@ Definition COMPS (t : COMPT) : compd :=
   | UserInput => mk_compd "UserInput" "test/quark/user-input.py" [] (mk_vdesc [])
   end.
 
+Definition IENVD : vdesc := mk_vdesc
+  [ fd_d (* curtab *)
+  ; fd_d (* screen *)
+  ; fd_d (* userinput *)
+  ].
+
+Definition KSTD : vdesc := mk_vdesc
+  [ fd_d (* curtab *)
+  ; fd_d (* screen *)
+  ; fd_d (* user-input *)
+  ].
+
+Notation curtab    := (None) (only parsing).
+Notation screen    := (Some None) (only parsing).
+Notation userinput := (Some (Some None)) (only parsing).
+
+End SystemFeatures.
+
+Import SystemFeatures.
+
+Module Language := MkLanguage(SystemFeatures).
+
+Import Language.
+
 Definition default_domain := str_of_string "google.com".
 
-Definition IMSG : msg PAYD := @Build_msg _ PAYD Quit tt.
+Module Spec : SpecInterface.
 
-Definition INIT : init_prog PAYD COMPT COMPS KSTD IMSG IENVD :=
-  [ fun s => Spawn _ _ COMPS _ _ IENVD Tab       (default_domain, tt) None (Logic.eq_refl _)
-  ; fun s => Spawn _ _ COMPS _ _ IENVD Screen    tt                   None (Logic.eq_refl _)
-  ; fun s => Spawn _ _ COMPS _ _ IENVD UserInput tt                   None (Logic.eq_refl _)
+Module FEATURES := SystemFeatures.
+
+Definition INIT : init_prog PAYD COMPT COMPS KSTD IENVD :=
+  [ fun s => spawn IENVD _ Tab       (default_domain, tt) None (Logic.eq_refl _)
+  ; fun s => spawn IENVD _ Screen    tt                   None (Logic.eq_refl _)
+  ; fun s => spawn IENVD _ UserInput tt                   None (Logic.eq_refl _)
   ].
 
 Definition HANDLERS : handlers PAYD COMPT COMPS KSTD :=
-  (fun m cfd =>
-    match tag PAYD m as _tm return
-      @sdenote _ SDenoted_vdesc (lkup_tag PAYD _tm) -> _
-    with
+  (fun m cc =>
+     let (_, cf, _) := cc in
+     match tag PAYD m as _tm return
+       @sdenote _ SDenoted_vdesc (lkup_tag PAYD _tm) -> _
+     with
 
-    | Input => fun pl =>
+     | Input => fun pl =>
        let envd := mk_vdesc [] in
-       existT (fun d => hdlr_prog PAYD COMPT COMPS KSTD m d) envd (
+       existT (fun d => hdlr_prog PAYD COMPT COMPS KSTD cc m d) envd (
          let (input, _) := pl in fun st0 =>
-         if fd_eq cfd (shvec_ith (n := projT1 KSTD) _
-                                 (projT2 KSTD) (kst _ _ _ _ st0) userinput)
-         then
-           [ fun s => Send PAYD COMPT COMPS KSTD _ envd
-                           (StVar _ KSTD m _ curtab) Input
-                           (SLit _ _ m _  input, tt) ]
-         else
-           []
-       )
-
-    | Display => fun pl =>
-       let envd := mk_vdesc [] in
-       existT (fun d => hdlr_prog PAYD COMPT COMPS KSTD m d) envd (
-         let (url, _) := pl in fun st0 =>
-         if fd_eq cfd (shvec_ith (n := projT1 KSTD) _
-                                 (projT2 KSTD) (kst _ _ _ _ st0) curtab)
-         then
-           [ fun s => Send PAYD COMPT COMPS KSTD _ envd
-                           (StVar _ KSTD m _ screen) Display
-                           (SLit _ _ m _ url, tt) ]
-         else
-           []
-       )
-
-    | Quit => fun pl =>
-       let envd := mk_vdesc [] in
-       existT (fun d => hdlr_prog PAYD COMPT COMPS KSTD m d) envd (
-         let _ := pl in fun st0 =>
          if fd_eq
-              cfd
+              cf
               (shvec_ith (n := projT1 KSTD) _ (projT2 KSTD) (kst _ _ _ _ st0) userinput)
          then
-           [ fun s => Send PAYD COMPT COMPS KSTD _ envd
-                           (StVar _ KSTD m _ curtab) Quit tt
-           ; fun s => Send PAYD COMPT COMPS KSTD _ envd
-                           (StVar _ KSTD m _ screen) Quit tt
+           [ fun s => sendall envd _
+                       (Build_comp_pat COMPT' COMPS Tab
+                         (Some (shvec_ith (n := projT1 KSTD) _ (projT2 KSTD)
+                                          (kst _ _ _ _ st0) curtab))
+                         (None, tt))
+                       Input (slit input, tt)
            ]
          else
            []
        )
 
-    | Some (Some (Some bad)) => fun _ =>
-      match bad with end
+     | Display => fun pl =>
+       let envd := mk_vdesc [] in
+       existT (fun d => hdlr_prog PAYD COMPT COMPS KSTD cc m d) envd (
+         let (url, _) := pl in fun st0 =>
+         if fd_eq
+              cf
+              (shvec_ith (n := projT1 KSTD) _ (projT2 KSTD) (kst _ _ _ _ st0) curtab)
+         then
+           [ fun s => sendall envd _
+                       (Build_comp_pat COMPT' COMPS Screen
+                         (Some (shvec_ith (n := projT1 KSTD) _ (projT2 KSTD)
+                                          (kst _ _ _ _ st0) screen))
+                         tt)
+                       Display (slit url, tt)
+           ]
+         else
+           []
+       )
+
+     | Quit => fun pl =>
+       let envd := mk_vdesc [] in
+       existT (fun d => hdlr_prog PAYD COMPT COMPS KSTD cc m d) envd (
+         let _ := pl in fun st0 =>
+         if fd_eq
+              cf
+              (shvec_ith (n := projT1 KSTD) _ (projT2 KSTD) (kst _ _ _ _ st0) userinput)
+         then
+           [ fun s => sendall envd _
+                       (Build_comp_pat COMPT' COMPS Tab
+                         (Some (shvec_ith (n := projT1 KSTD) _ (projT2 KSTD)
+                                          (kst _ _ _ _ st0) curtab))
+                         (None, tt))
+                       Quit tt
+           ; fun s => sendall envd _
+                       (Build_comp_pat COMPT' COMPS Screen
+                         (Some (shvec_ith (n := projT1 KSTD) _ (projT2 KSTD)
+                                          (kst _ _ _ _ st0) screen))
+                         tt)
+                       Quit tt
+           ]
+         else
+           []
+       )
+
+     | Some (Some (Some bad)) => fun _ =>
+       match bad with end
     end (pay PAYD m)
   ).
 
-Definition main := mk_main (Build_spec NB_MSG PAYD IENVD KSTD COMPT COMPTDEC COMPS IMSG INIT HANDLERS).
+End Spec.
+
+Module Main := MkMain(Spec).
+Import Main.
