compiler/dsl/coq/ReflexSSH.v
@@ -16,19 +16,19 @@ Open Scope string_scope.
  2) MON waits till SLV sends LoginReq
 
  == Login Request
- 1) SLV asks MON to login via LoginReq, 
+ 1) SLV asks MON to login via LoginReq,
  1-1) if login_cnt =n 3 then send Login_Res(0) back to SLV
- 1-2) otherwise, login_cnt = login_cnt + 1, then send SysLogReq() 
+ 1-2) otherwise, login_cnt = login_cnt + 1, then send SysLogReq()
  to SYS
 
- 2) SYS replies to MON with SysLogRes() 
- if the response is 1 then set login_succeded = 1; and 
- login_account = $account and MON delivers it to SLV with LogRes  
+ 2) SYS replies to MON with SysLogRes()
+ if the response is 1 then set login_succeded = 1; and
+ login_account = $account and MON delivers it to SLV with LogRes
 
  == PubKey Request
  1) SLV asks MON for the public key via PubKeyReq
  MON delivers it to SYS via SysPubKeyReq
-  
+
  2) SYS replies to MON with SysPubKeyRes
  MON delivers it to SLV
 
@@ -37,22 +37,24 @@ Open Scope string_scope.
 
  == CreatePtyer
  1) SLV asks MON for a created PTYER
- 1-1) if login_succeeded =n 0 then ignore this request completely 
+ 1-1) if login_succeeded =n 0 then ignore this request completely
  and don't send anything back
 
  2) MON creates a PTY by sending SysCreatePtyReq()
- 3) SYS sends back with SysCreatPtyRes(fdesc, fdesc) 
+ 3) SYS sends back with SysCreatPtyRes(fdesc, fdesc)
  (SYS applies ioctl() to the slave fd & it creates a ptyer inside it
  (Question: there are two options : a. create ptyer inside SYS
- b. spawns a ptyer as a component from MON. Which one is better?? ) 
+ b. spawns a ptyer as a component from MON. Which one is better?? )
 
  4) MON replies back to SLV with the two file descriptors
 *)
 
+Module SystemFeatures <: SystemFeaturesInterface.
+
 Definition NB_MSG : nat := 18.
 
 Definition PAYD : vvdesc NB_MSG := mk_vvdesc
-  [ 
+  [
     (* slave <- monitor *)
     ("LoginReq",   [str_d]);
     ("LoginResT",   []);
@@ -81,61 +83,10 @@ Definition PAYD : vvdesc NB_MSG := mk_vvdesc
     ("SCreatePtyerReq",   [str_d]);
     ("SCreatePtyerRes",   [fd_d; fd_d])
   ].
- 
-Notation LoginReq :=       (None) (only parsing).
-Notation LoginResT :=      (Some None) (only parsing).
-Notation LoginResF :=      (Some (Some None)) (only parsing).
-      
-Notation PubkeyReq :=      (Some (Some (Some None))) (only parsing).
-Notation PubkeyRes :=      (Some (Some (Some (Some None)))) (only parsing).
 
-Notation KeysignReq :=     (Some (Some (Some (Some (Some None))))) (only parsing).
-Notation KeysignRes :=     (Some (Some (Some (Some (Some (Some None)))))) (only parsing).
+Inductive COMPT' : Type := System | Slave.
 
-Notation CreatePtyerReq := (Some (Some (Some (Some (Some (Some (Some None))))))) (only parsing).
-Notation CreatePtyerRes := (Some (Some (Some (Some (Some (Some (Some (Some None)))))))) (only parsing).
-
-    (* monitor <-> system *)
-Notation SLoginReq :=      (Some (Some (Some (Some (Some (Some (Some (Some (Some None))))))))) (only parsing).
-Notation SLoginResT :=     (Some (Some (Some (Some (Some (Some (Some (Some (Some (Some None)))))))))) (only parsing).
-Notation SLoginResF :=     (Some (Some (Some (Some (Some (Some (Some (Some (Some (Some (Some None))))))))))) (only parsing).
-
-Notation SPubkeyReq :=     (Some (Some (Some (Some (Some (Some (Some (Some (Some (Some (Some (Some None)))))))))))) (only parsing).
-Notation SPubkeyRes :=     (Some (Some (Some (Some (Some (Some (Some (Some (Some (Some (Some (Some (Some None))))))))))))) (only parsing).
-
-Notation SKeysignReq :=    (Some (Some (Some (Some (Some (Some (Some (Some (Some (Some (Some (Some (Some (Some None)))))))))))))) (only parsing).
-Notation SKeysignRes :=    (Some (Some (Some (Some (Some (Some (Some (Some (Some (Some (Some (Some (Some (Some (Some None))))))))))))))) (only parsing).
-
-Notation SCreatePtyerReq := (Some (Some (Some (Some (Some (Some (Some (Some (Some (Some (Some (Some (Some (Some (Some (Some None)))))))))))))))) (only parsing).
-Notation SCreatePtyerRes := (Some (Some (Some (Some (Some (Some (Some (Some (Some (Some (Some (Some (Some (Some (Some (Some (Some None))))))))))))))))) (only parsing).
-
-
-Definition KSTD : vdesc := mk_vdesc
-  [ fd_d (* system *)
-  ; fd_d (* slave *)
-  ; num_d (* authenticated *)
-  ; str_d (* authenticated username *)
-  ].
-
-Notation v_st_system := (None) (only parsing).
-Notation v_st_slave := (Some None) (only parsing).
-Notation v_st_authenticated := (Some (Some None)) (only parsing).
-Notation v_st_auth_user := (Some (Some (Some None))) (only parsing).
-
-Notation system := (StVar _ KSTD _ _ v_st_system) (only parsing).
-Notation slave := (StVar _ KSTD _ _ v_st_slave) (only parsing).
-Notation authenticated := (StVar _ KSTD _ _ v_st_authenticated) (only parsing).
-Notation auth_user := (StVar _ KSTD _ _ v_st_auth_user) (only parsing).
-
-Definition IENVD : vdesc := mk_vdesc
-  [ fd_d (* system *)
-  ; fd_d (* slave *)
-  ].
-
-Notation v_env_system := (None) (only parsing).
-Notation v_env_slave := (Some None) (only parsing).
-
-Inductive COMPT : Type := System | Slave.
+Definition COMPT := COMPT'.
 
 Definition COMPTDEC : forall (x y : COMPT), decide (x = y).
 Proof. decide equality. Defined.
@@ -150,13 +101,60 @@ Definition COMPS (t : COMPT) : compd :=
                 (mk_vdesc [])
   end.
 
-Definition IMSG : msg PAYD := @Build_msg _ PAYD LoginReq (str_of_string "", tt).
+Notation LoginReq  := (None) (only parsing).
+Notation LoginResT := (Some None) (only parsing).
+Notation LoginResF := (Some (Some None)) (only parsing).
+Notation PubkeyReq :=      (Some (Some (Some None))) (only parsing).
+Notation PubkeyRes :=      (Some (Some (Some (Some None)))) (only parsing).
+Notation KeysignReq :=     (Some (Some (Some (Some (Some None))))) (only parsing).
+Notation KeysignRes :=     (Some (Some (Some (Some (Some (Some None)))))) (only parsing).
+Notation CreatePtyerReq := (Some (Some (Some (Some (Some (Some (Some None))))))) (only parsing).
+Notation CreatePtyerRes := (Some (Some (Some (Some (Some (Some (Some (Some None)))))))) (only parsing).
+Notation SLoginReq :=      (Some (Some (Some (Some (Some (Some (Some (Some (Some None))))))))) (only parsing).
+Notation SLoginResT :=     (Some (Some (Some (Some (Some (Some (Some (Some (Some (Some None)))))))))) (only parsing).
+Notation SLoginResF :=     (Some (Some (Some (Some (Some (Some (Some (Some (Some (Some (Some None))))))))))) (only parsing).
+Notation SPubkeyReq :=     (Some (Some (Some (Some (Some (Some (Some (Some (Some (Some (Some (Some None)))))))))))) (only parsing).
+Notation SPubkeyRes :=     (Some (Some (Some (Some (Some (Some (Some (Some (Some (Some (Some (Some (Some None))))))))))))) (only parsing).
+Notation SKeysignReq :=    (Some (Some (Some (Some (Some (Some (Some (Some (Some (Some (Some (Some (Some (Some None)))))))))))))) (only parsing).
+Notation SKeysignRes :=    (Some (Some (Some (Some (Some (Some (Some (Some (Some (Some (Some (Some (Some (Some (Some None))))))))))))))) (only parsing).
+Notation SCreatePtyerReq := (Some (Some (Some (Some (Some (Some (Some (Some (Some (Some (Some (Some (Some (Some (Some (Some None)))))))))))))))) (only parsing).
+Notation SCreatePtyerRes := (Some (Some (Some (Some (Some (Some (Some (Some (Some (Some (Some (Some (Some (Some (Some (Some (Some None))))))))))))))))) (only parsing).
 
-Definition INIT : init_prog PAYD COMPT COMPS KSTD IMSG IENVD :=
-  [ fun s => Spawn _ _ COMPS _ _ IENVD System (str_of_string "System", tt)
-                   v_env_system (Logic.eq_refl _)
-  ; fun s => Spawn _ _ COMPS _ _ IENVD Slave tt
-                   v_env_slave (Logic.eq_refl _)
+Definition IENVD : vdesc := mk_vdesc
+  [ fd_d (* system *)
+  ; fd_d (* slave *)
+  ].
+
+Notation v_env_system := (None) (only parsing).
+Notation v_env_slave := (Some None) (only parsing).
+
+Definition KSTD : vdesc := mk_vdesc
+  [ fd_d (* system *)
+  ; fd_d (* slave *)
+  ; num_d (* authenticated *)
+  ; str_d (* authenticated username *)
+  ].
+
+Notation v_st_system := (None) (only parsing).
+Notation v_st_slave := (Some None) (only parsing).
+Notation v_st_authenticated := (Some (Some None)) (only parsing).
+Notation v_st_auth_user := (Some (Some (Some None))) (only parsing).
+
+End SystemFeatures.
+
+Import SystemFeatures.
+
+Module Language := MkLanguage(SystemFeatures).
+
+Import Language.
+
+Module Spec : SpecInterface.
+
+Module FEATURES := SystemFeatures.
+
+Definition INIT : init_prog PAYD COMPT COMPS KSTD IENVD :=
+  [ fun s => spawn IENVD _ System (str_of_string "System", tt) v_env_system (Logic.eq_refl _)
+  ; fun s => spawn IENVD _ Slave  tt                           v_env_slave  (Logic.eq_refl _)
   ].
 
 Definition system_pat := (Some (str_of_string "System"), tt).
@@ -164,178 +162,209 @@ Definition system_pat := (Some (str_of_string "System"), tt).
 Definition exists_comp := exists_comp COMPT COMPTDEC COMPS.
 
 Definition HANDLERS : handlers PAYD COMPT COMPS KSTD :=
-  (fun m cfd =>
-    match tag PAYD m as _tm return
-      @sdenote _ SDenoted_vdesc (lkup_tag PAYD _tm) -> _
-    with
-      (* login *)
+  (fun m cc =>
+     let (_, cf, _) := cc in
+     match tag PAYD m as _tm return
+       @sdenote _ SDenoted_vdesc (lkup_tag PAYD _tm) -> _
+     with
 
-    | LoginReq => fun pl =>
+     | LoginReq => fun pl =>
        let envd := mk_vdesc [] in
-       existT (fun d => hdlr_prog PAYD COMPT COMPS KSTD _ d) envd (
+       existT (fun d => hdlr_prog PAYD COMPT COMPS KSTD cc _ d) envd (
          let (loginstr, _) := pl in
          (fun st0 =>
-            [ fun s => Send PAYD _ _ _ _ _ system
-                            SLoginReq (SLit _ _ _ _ loginstr, tt)
+            [ fun s => sendall envd _
+                       (Build_comp_pat COMPT' COMPS System
+                         (Some (shvec_ith (n := projT1 KSTD) _ (projT2 KSTD)
+                                          (kst _ _ _ _ st0) v_st_system))
+                         (None, tt))
+                       SLoginReq (slit loginstr, tt)
             ]
          )
        )
 
-    | SLoginResT => fun pl =>
+     | SLoginResT => fun pl =>
        let envd := mk_vdesc [] in
-       existT (fun d => hdlr_prog PAYD COMPT COMPS KSTD _ d) envd (
-         let (user, _) := pl in           
+       existT (fun d => hdlr_prog PAYD COMPT COMPS KSTD cc _ d) envd (
+         let (user, _) := pl in
          (fun st0 =>
-            if exists_comp (Build_comp_pat COMPT COMPS System (Some cfd) system_pat) (kcs _ _ _ _ st0)
+            if exists_comp
+                 (Build_comp_pat COMPT COMPS System (Some cf) system_pat)
+                 (kcs _ _ _ _ st0)
             then
-            [ 
-              
-              fun s => StUpd PAYD _ COMPS KSTD _ _ v_st_auth_user
-                             strd_neq_fdd (SLit _ _ _ _ user); 
-              fun s => StUpd PAYD _ _ KSTD _ _ v_st_authenticated
-                             numd_neq_fdd (NLit _ _ _ _ (num_of_nat 1));
-              fun s => Send PAYD _ _ _ _ _ slave LoginResT tt
+            [ fun s => stupd envd _ v_st_auth_user     (slit user)
+            ; fun s => stupd envd _ v_st_authenticated (nlit (num_of_nat 1))
+            ; fun s => sendall envd _
+                       (Build_comp_pat COMPT' COMPS Slave
+                         (Some (shvec_ith (n := projT1 KSTD) _ (projT2 KSTD)
+                                          (kst _ _ _ _ st0) v_st_slave))
+                         tt)
+                       LoginResT tt
             ]
             else []
          )
        )
 
-    | SLoginResF => fun pl =>
+     | SLoginResF => fun pl =>
        let envd := mk_vdesc [] in
-       existT (fun d => hdlr_prog PAYD COMPT COMPS KSTD _ d) envd (
+       existT (fun d => hdlr_prog PAYD COMPT COMPS KSTD cc _ d) envd (
          (fun st0 =>
-            [ fun s => Send PAYD _ _ _ _ _ slave LoginResF tt
+            [ fun s => sendall envd _
+                       (Build_comp_pat COMPT' COMPS Slave
+                         (Some (shvec_ith (n := projT1 KSTD) _ (projT2 KSTD)
+                                          (kst _ _ _ _ st0) v_st_slave))
+                         tt)
+                       LoginResF tt
             ]
          )
        )
 
-       (* pub key request *)
-
-    | PubkeyReq => fun pl =>
+     | PubkeyReq => fun pl =>
        let envd := mk_vdesc [] in
-       existT (fun d => hdlr_prog PAYD COMPT COMPS KSTD _ d) envd (
+       existT (fun d => hdlr_prog PAYD COMPT COMPS KSTD cc _ d) envd (
          (fun st0 =>
-            [ fun s => Send PAYD _ _ _ _ _ system SPubkeyReq tt
+            [ fun s => sendall envd _
+                       (Build_comp_pat COMPT' COMPS System
+                         (Some (shvec_ith (n := projT1 KSTD) _ (projT2 KSTD)
+                                          (kst _ _ _ _ st0) v_st_system))
+                         (None, tt))
+                       SPubkeyReq tt
             ]
          )
        )
 
-    | SPubkeyRes => fun pl =>
+     | SPubkeyRes => fun pl =>
        let envd := mk_vdesc [] in
-       existT (fun d => hdlr_prog PAYD COMPT COMPS KSTD _ d) envd (
+       existT (fun d => hdlr_prog PAYD COMPT COMPS KSTD cc _ d) envd (
          let (pubkey, _) := pl in
          (fun st0 =>
-            [ fun s => Send PAYD _ _ _ _ _ system
-                            SPubkeyRes (SLit _ _ _ _ pubkey, tt)
+            [ fun s => sendall envd _
+                       (Build_comp_pat COMPT' COMPS System
+                         (Some (shvec_ith (n := projT1 KSTD) _ (projT2 KSTD)
+                                          (kst _ _ _ _ st0) v_st_system))
+                         (None, tt))
+                       SPubkeyRes (slit pubkey, tt)
             ]
          )
        )
-       
-       (* key sign *)
 
-    | KeysignReq => fun pl =>
+     | KeysignReq => fun pl =>
        let envd := mk_vdesc [] in
-       existT (fun d => hdlr_prog PAYD COMPT COMPS KSTD _ d) envd (
+       existT (fun d => hdlr_prog PAYD COMPT COMPS KSTD cc _ d) envd (
          let (keystr, _) := pl in
          (fun st0 =>
-            [ fun s => Send PAYD _ _ _ _ _ system
-                            SKeysignReq (SLit _ _ _ _ keystr, tt)
+            [ fun s => sendall envd _
+                       (Build_comp_pat COMPT' COMPS System
+                         (Some (shvec_ith (n := projT1 KSTD) _ (projT2 KSTD)
+                                          (kst _ _ _ _ st0) v_st_system))
+                         (None, tt))
+                       SKeysignReq (slit keystr, tt)
             ]
          )
        )
 
-    | SKeysignRes => fun pl =>
+     | SKeysignRes => fun pl =>
        let envd := mk_vdesc [] in
-       existT (fun d => hdlr_prog PAYD COMPT COMPS KSTD _ d) envd (
+       existT (fun d => hdlr_prog PAYD COMPT COMPS KSTD cc _ d) envd (
          let (signedkey, _) := pl in
          (fun st0 =>
-            [ fun s => Send PAYD _ _ _ _ _ system
-                            KeysignRes (SLit _ _ _ _ signedkey, tt)
+            [ fun s => sendall envd _
+                       (Build_comp_pat COMPT' COMPS System
+                         (Some (shvec_ith (n := projT1 KSTD) _ (projT2 KSTD)
+                                          (kst _ _ _ _ st0) v_st_system))
+                         (None, tt))
+                       KeysignRes (slit signedkey, tt)
             ]
          )
        )
 
-       (* create pseudo terminal *)
-
-    | CreatePtyerReq => fun pl =>
+     | CreatePtyerReq => fun pl =>
        let envd := mk_vdesc [] in
-       existT (fun d => hdlr_prog PAYD COMPT COMPS KSTD _ d) envd (
+       existT (fun d => hdlr_prog PAYD COMPT COMPS KSTD cc _ d) envd (
          (fun st0 =>
            if num_eq
                 (shvec_ith _ (projT2 KSTD:svec desc 4) (kst _ _ _ _ st0) v_st_authenticated)
                 (num_of_nat 0)
            then []
-           else [ 
-               fun s => Send PAYD _ _ _ _ _ system
-                             SCreatePtyerReq (auth_user,tt)
-             ]
+           else [ fun s => sendall envd _
+                            (Build_comp_pat COMPT' COMPS System
+                              (Some (shvec_ith (n := projT1 KSTD) _ (projT2 KSTD)
+                                               (kst _ _ _ _ st0) v_st_system))
+                              (None, tt))
+                            SCreatePtyerReq (stvar v_st_auth_user, tt)
+                ]
          )
        )
 
-    | SCreatePtyerRes => fun pl =>
+     | SCreatePtyerRes => fun pl =>
        let envd := mk_vdesc [] in
-       existT (fun d => hdlr_prog PAYD COMPT COMPS KSTD _ d) envd (
-         match pl with 
-           | (fd0, (fd1, _)) =>
-             (fun st0 =>
-               [ fun s => Send PAYD _ _ _ _ _
-                               system CreatePtyerRes
-                               (CFd PAYD _ _ _, (CFd PAYD _ _ _, tt))
-               ]
-             )
+       existT (fun d => hdlr_prog PAYD COMPT COMPS KSTD cc _ d) envd (
+         match pl with
+         | (fd0, (fd1, _)) =>
+           (fun st0 =>
+              [ fun s => sendall envd _
+                            (Build_comp_pat COMPT' COMPS System
+                              (Some (shvec_ith (n := projT1 KSTD) _ (projT2 KSTD)
+                                               (kst _ _ _ _ st0) v_st_system))
+                              (None, tt))
+                            CreatePtyerRes (cfd, (cfd, tt))
+              ]
+           )
          end
        )
-       
 
-       (* not meant to be received by the kernel *)
-    | LoginResT => fun pl =>
+     (* not meant to be received by the kernel *)
+     | LoginResT => fun pl =>
        let envd := mk_vdesc [] in
-       existT (fun d => hdlr_prog PAYD COMPT COMPS KSTD _ d) envd (
+       existT (fun d => hdlr_prog PAYD COMPT COMPS KSTD cc _ d) envd (
          (fun st0 => [])
        )
-    | LoginResF => fun pl =>
+     | LoginResF => fun pl =>
        let envd := mk_vdesc [] in
-       existT (fun d => hdlr_prog PAYD COMPT COMPS KSTD _ d) envd (
+       existT (fun d => hdlr_prog PAYD COMPT COMPS KSTD cc _ d) envd (
          (fun st0 => [])
        )
-    | PubkeyRes => fun pl =>
+     | PubkeyRes => fun pl =>
        let envd := mk_vdesc [] in
-       existT (fun d => hdlr_prog PAYD COMPT COMPS KSTD _ d) envd (
+       existT (fun d => hdlr_prog PAYD COMPT COMPS KSTD cc _ d) envd (
          (fun st0 => [])
        )
-    | KeysignRes => fun pl =>
+     | KeysignRes => fun pl =>
        let envd := mk_vdesc [] in
-       existT (fun d => hdlr_prog PAYD COMPT COMPS KSTD _ d) envd (
+       existT (fun d => hdlr_prog PAYD COMPT COMPS KSTD cc _ d) envd (
          (fun st0 => [])
        )
-    | CreatePtyerRes => fun pl =>
+     | CreatePtyerRes => fun pl =>
        let envd := mk_vdesc [] in
-       existT (fun d => hdlr_prog PAYD COMPT COMPS KSTD _ d) envd (
+       existT (fun d => hdlr_prog PAYD COMPT COMPS KSTD cc _ d) envd (
          (fun st0 => [])
        )
-    | SLoginReq => fun pl =>
+     | SLoginReq => fun pl =>
        let envd := mk_vdesc [] in
-       existT (fun d => hdlr_prog PAYD COMPT COMPS KSTD _ d) envd (
+       existT (fun d => hdlr_prog PAYD COMPT COMPS KSTD cc _ d) envd (
          (fun st0 => [])
        )
-    | SPubkeyReq => fun pl =>
+     | SPubkeyReq => fun pl =>
        let envd := mk_vdesc [] in
-       existT (fun d => hdlr_prog PAYD COMPT COMPS KSTD _ d) envd (
+       existT (fun d => hdlr_prog PAYD COMPT COMPS KSTD cc _ d) envd (
          (fun st0 => [])
        )
-    | SKeysignReq => fun pl =>
+     | SKeysignReq => fun pl =>
        let envd := mk_vdesc [] in
-       existT (fun d => hdlr_prog PAYD COMPT COMPS KSTD _ d) envd (
+       existT (fun d => hdlr_prog PAYD COMPT COMPS KSTD cc _ d) envd (
          (fun st0 => [])
        )
-    | SCreatePtyerReq => fun pl =>
+     | SCreatePtyerReq => fun pl =>
        let envd := mk_vdesc [] in
-       existT (fun d => hdlr_prog PAYD COMPT COMPS KSTD _ d) envd (
+       existT (fun d => hdlr_prog PAYD COMPT COMPS KSTD cc _ d) envd (
          (fun st0 => [])
        )
-    | (Some (Some (Some (Some (Some (Some (Some (Some (Some (Some (Some (Some (Some (Some (Some (Some (Some (Some bad)))))))))))))))))) => fun _ =>
+     | (Some (Some (Some (Some (Some (Some (Some (Some (Some (Some (Some (Some (Some (Some (Some (Some (Some (Some bad)))))))))))))))))) => fun _ =>
       match bad with end
     end (pay PAYD m)
   ).
 
-Definition main := mk_main (Build_spec NB_MSG PAYD IENVD KSTD COMPT COMPTDEC COMPS IMSG INIT HANDLERS).
+End Spec.
+
+Module Main := MkMain(Spec).
+Import Main.
