compiler/pollang/ActionMatch.v
@@ -9,6 +9,10 @@ Section KOAction.
 
 Context {NB_MSG : nat}.
 Variable PAYD : vvdesc NB_MSG.
+Variable COMPT : Set.
+Variable COMPS : COMPT -> compd.
+Variable COMPTDEC : forall (x y : COMPT), decide (x = y).
+Definition comp_pat := comp_pat COMPT COMPS.
 
 Definition soptdenote_desc (d : desc) : Set :=
   option (sdenote_desc d).
@@ -21,15 +25,40 @@ Record opt_msg : Set :=
 Inductive KOAction : Set :=
 | KOExec   : option str -> option (list (option str)) -> option fd -> KOAction
 | KOCall   : option str -> option (list (option str)) -> option fd -> KOAction
-| KOSelect : option (list (option fd)) -> option fd -> KOAction
-| KOSend   : option fd -> option opt_msg -> KOAction
-| KORecv   : option fd -> option opt_msg -> KOAction
-| KOBogus  : option fd -> option num -> KOAction.
+| KOSelect : option (list (option comp_pat)) -> option comp_pat -> KOAction
+| KOSend   : option comp_pat -> option opt_msg -> KOAction
+| KORecv   : option comp_pat -> option opt_msg -> KOAction
+| KOBogus  : option comp_pat -> option num -> KOAction.
 
 Definition eltMatch (d:desc) (opt:option s[[d]]) (arg:s[[d]]) : Prop :=
   match opt with
   | None   => True
   | Some t => t = arg
+  end.
+
+Definition match_comp' (cp : comp_pat) (c : comp COMPT COMPS) : Prop :=
+  match c, cp with
+  | Build_comp t f cfg, Build_comp_pat t' fp cfgp =>
+    match COMPTDEC t t' with
+    | left EQ =>
+      match fp with None => True | Some f' => f = f' end
+      /\
+      match EQ in _ = _t return
+        shvec sdenote_desc_cfg_pat (projT2 (comp_conf_desc _ _ _t)) -> Prop
+      with
+      | Logic.eq_refl => fun cfgp =>
+        shvec_match_prop (projT2 (comp_conf_desc _ _ t))
+                         soptdenote_desc sdenote_desc
+                         eltMatch cfgp cfg
+      end cfgp
+    | right _ => False
+    end
+  end.
+
+Definition match_comp (cpopt:option comp_pat) (c:comp COMPT COMPS) : Prop :=
+  match cpopt with
+  | None    => True
+  | Some cp => match_comp' cp c
   end.
 
 Definition msgMatch' (optm:opt_msg) (m:msg PAYD) : Prop :=
@@ -68,7 +97,22 @@ Definition listMatch (d:desc)
   | Some lopt' => listMatch' d lopt' l
   end.
 
-Definition AMatch (oact:KOAction) (act:KAction PAYD) : Prop :=
+Fixpoint comp_list_match'
+  (lopt:list (option comp_pat)) (l:list (comp COMPT COMPS)) :=
+  match lopt, l with
+  | nil, nil          => True
+  | cpopt::lopt', c::l' => match_comp cpopt c /\ comp_list_match' lopt' l'
+  | _, _              => False
+  end.
+
+Definition comp_list_match
+  (lopt:option (list (option comp_pat))) (l:list (comp COMPT COMPS)) :=
+  match lopt with
+  | None => True
+  | Some lopt' => comp_list_match' lopt' l
+  end.
+
+Definition AMatch (oact:KOAction) (act:KAction PAYD COMPT COMPS) : Prop :=
 match oact, act with
 | KOExec s ls f, KExec s' ls' f' => eltMatch str_d s s' /\
                                     listMatch str_d ls ls'  /\
@@ -76,15 +120,15 @@ match oact, act with
 | KOCall s ls f, KCall s' ls' f' => eltMatch str_d s s' /\
                                     listMatch str_d ls ls' /\
                                     eltMatch fd_d f f'
-| KOSelect lfd f, KSelect lfd' f' => listMatch fd_d lfd lfd' /\
-                                     eltMatch fd_d f f'
-| KOSend f omsg, KSend f' amsg => eltMatch fd_d f f' /\
+| KOSelect lcps cp, KSelect lcs c => comp_list_match lcps lcs /\
+                                     match_comp cp c
+| KOSend cp omsg, KSend c amsg => match_comp cp c /\
                                   msgMatch omsg amsg
-| KORecv f omsg, KRecv f' amsg => eltMatch fd_d f f' /\
+| KORecv cp omsg, KRecv c amsg => match_comp cp c /\
                                   msgMatch omsg amsg
 (**I don't know if this is the right thing to do for KBogus matching.
    It just checks if the message tags and fds are the same**)
-| KOBogus f optbtag, KBogus f' bmsg => eltMatch fd_d f f' /\
+| KOBogus cp optbtag, KBogus c bmsg => match_comp cp c /\
                                        eltMatch num_d optbtag (btag bmsg)
 | _, _ => False
 end.
@@ -104,6 +148,47 @@ Proof.
   destruct oelt;
   [ destruct d; [apply num_eq | apply str_eq | apply fd_eq]
   | auto].
+Qed.
+
+Definition decide_shvec_match :
+  forall n (vd:svec desc n) v v',
+    decide (shvec_match_prop vd soptdenote_desc sdenote_desc eltMatch v v').
+Proof.
+  intros n vd v v'.
+  induction n; auto.
+      simpl in *.
+      destruct vd as [d vd'].
+      destruct v as [oelt orest].
+      destruct v' as [elt rest].
+      apply decide_and; [apply decide_elt_match | auto].
+Qed.
+
+Definition decide_match_comp :
+  forall COMPT COMPS COMPTDEC cpopt c,
+    decide (match_comp COMPT COMPS COMPTDEC cpopt c).
+Proof.
+  intros COMPT COMPS COMPTDEC cpopt c.
+  destruct cpopt as [cp | ]; [simpl; destruct cp; destruct c | auto].
+    unfold match_comp'.
+    match goal with
+    |- context[COMPTDEC ?comp_type ?comp_pat_type]
+      => destruct (COMPTDEC comp_type comp_pat_type) as [eq | ];
+         [destruct eq | auto]
+    end.
+
+    destruct comp_pat_fd;
+      [apply decide_and; [apply fd_eq | apply decide_shvec_match]
+      | apply decide_and; [auto | apply decide_shvec_match] ].
+Qed.
+
+Definition decide_list_match_comp :
+  forall COMPT COMPS COMPTDEC lopt l,
+    decide (comp_list_match COMPT COMPS COMPTDEC lopt l).
+Proof.
+  intros COMPT COMPS COMPTDEC lopt l.
+  destruct lopt as [lopt' | ]; simpl; auto.
+    generalize dependent l; induction lopt'; destruct l; simpl; auto.
+      apply decide_and; [apply decide_match_comp | apply IHlopt'].
 Qed.
 
 Definition decide_list_match : forall d lopt l,
@@ -129,23 +214,21 @@ Proof.
     end.
     destruct m as [tag pay]; simpl in *.
     destruct (lkup_tag PAYD tag) as [n vd].
-    induction n; auto.
-      simpl in *.
-      destruct vd as [d vd'].
-      destruct opay as [oelt orest].
-      destruct pay as [elt rest].
-      apply decide_and; [apply decide_elt_match | auto].
+    apply decide_shvec_match.
 Qed.
 
-Definition decide_act : forall {NB_MSG} (PAYD:vvdesc NB_MSG) oact act,
-                          decide (AMatch PAYD oact act).
+Definition decide_act :
+  forall {NB_MSG} (PAYD:vvdesc NB_MSG) COMPT COMPS COMPTDEC oact act,
+    decide (AMatch PAYD COMPT COMPS COMPTDEC oact act).
 Proof.
-  intros NB_MSG PAYD oact act.
+  intros NB_MSG PAYD COMPT COMPS COMPTDEC oact act.
   destruct oact; destruct act; simpl; auto; (*Takes care of decide (False)*)
   repeat apply decide_and;
   match goal with
   | [ |- decide (eltMatch _ _ _) ] => apply decide_elt_match
   | [ |- decide (listMatch _ _ _) ] => apply decide_list_match
   | [ |- decide (msgMatch _ _ _) ] => apply decide_msg_match
+  | [ |- decide (match_comp _ _ _ _ _) ] => apply decide_match_comp
+  | [ |- decide (comp_list_match _ _ _ _ _) ] => apply decide_list_match_comp
   end.
 Qed.
