compiler/dsl/coq/ReflexFrontend.v
@@ -2,22 +2,44 @@ Require Import String.
 
 Require Import Reflex.
 Require Import ReflexBase.
+Require Import ReflexFin.
 
-Record spec :=
-{ NB_MSG   : nat
-; PAYD     : vvdesc NB_MSG
-; IENVD    : vdesc
-; KSTD     : vdesc
-; COMPT    : Set
-; COMPTDEC : forall (x y : COMPT), decide (x = y)
-; COMPS    : COMPT -> compd
-; IMSG     : msg PAYD
-; INIT     : init_prog PAYD COMPT COMPS KSTD IMSG IENVD
-; HANDLERS : handlers PAYD COMPT COMPS KSTD
-}.
+Module Type SystemFeaturesInterface.
+  Parameter NB_MSG   : nat.
+  Parameter PAYD     : vvdesc NB_MSG.
+  Parameter COMPT    : Set.
+  Parameter COMPTDEC : forall (x y : COMPT), decide (x = y).
+  Parameter COMPS    : COMPT -> compd.
+  Parameter IENVD    : vdesc.
+  Parameter KSTD     : vdesc.
+End SystemFeaturesInterface.
 
-Definition mk_main (s : spec) :=
-  @main _ (PAYD s) (COMPT s) (COMPTDEC s) (COMPS s) (KSTD s) (IENVD s) (IMSG s) (INIT s) (HANDLERS s).
+Module MkLanguage (Import SF : SystemFeaturesInterface).
+  Definition sendall  := SendAll  PAYD COMPT COMPS KSTD.
+  Definition spawn := Spawn PAYD COMPT COMPS KSTD.
+  Definition stupd := StUpd PAYD COMPT COMPS KSTD.
+  Definition stvar {cc envd m} v :=
+    Term (hdlr_term PAYD COMPT COMPS KSTD cc m envd) (StVar _ _ _ _ _ _ _ v).
+  Definition slit {cc envd m} v :=
+    Term (hdlr_term PAYD COMPT COMPS KSTD cc m envd) (Base _ _ _ _ _ _ _ (SLit _ v)).
+  Definition nlit {cc envd m} v :=
+    Term (hdlr_term PAYD COMPT COMPS KSTD cc m envd) (Base _ _ _ _ _ _ _ (NLit _ v)).
+  Definition cfd {cc envd m} :=
+    Term (hdlr_term PAYD COMPT COMPS KSTD cc m envd) (CFd _ _ _ _ _ _ _).
+  Definition i_slit v := Term (base_term IENVD) (SLit _ v).
+  Definition i_nlit v := Term (base_term IENVD) (NLit _ v).
+End MkLanguage.
+
+Module Type SpecInterface.
+  Include SystemFeaturesInterface.
+  Parameter INIT : init_prog PAYD COMPT COMPS KSTD IENVD.
+  Parameter HANDLERS : handlers PAYD COMPT COMPS KSTD.
+End SpecInterface.
+
+Module MkMain (Import S : SpecInterface).
+  Definition main :=
+    @main _ PAYD COMPT COMPTDEC COMPS KSTD IENVD INIT HANDLERS.
+End MkMain.
 
 Fixpoint mk_vdesc' l : vdesc' (List.length l) :=
   match l with
@@ -44,14 +66,17 @@ Notation " [ ] " := nil.
 Notation " [ x ] " := (cons x nil).
 Notation " [ x ; .. ; y ] " := (cons x .. (cons y nil) ..).
 
-Definition cast_m_expr {NB_MSG} {PAYD : vvdesc NB_MSG} {KSTD envd} {m : msg PAYD} {t p d}
-  (EQ : Build_msg PAYD t p = m) (e : expr PAYD KSTD (Build_msg PAYD t p) envd d)
-  : expr PAYD KSTD m envd d
+Definition cast_m_expr
+  {NB_MSG COMPT COMPS} {PAYD : vvdesc NB_MSG} {KSTD envd} {m : msg PAYD} {cc t p d}
+  (EQ : Build_msg PAYD t p = m)
+  (e : expr (hdlr_term PAYD COMPT COMPS KSTD cc (Build_msg PAYD t p) envd) d)
+  : expr (hdlr_term PAYD COMPT COMPS KSTD cc m envd) d
   :=
-  match EQ in _ = _m return expr _ _ _m _ _ with
+  match EQ in _ = _m return expr (hdlr_term _ _ _ _ _ _m _) _ with
   | Logic.eq_refl => e
   end.
 
-Definition mvar {NB_MSG} {PAYD : vvdesc NB_MSG} {KSTD envd} {m : msg PAYD} {t p}
+Definition mvar
+  {NB_MSG COMPT COMPS} {PAYD : vvdesc NB_MSG} {KSTD envd} {m : msg PAYD} {cc t p}
   (EQ : Build_msg PAYD t p = m) i :=
-  cast_m_expr EQ (MVar PAYD KSTD (Build_msg PAYD t p) envd i).
+  cast_m_expr EQ (Term _ (MVar PAYD COMPT COMPS KSTD cc (Build_msg PAYD t p) envd i)).
