compiler/pollang/EchoPolicies.v
@@ -1,26 +1,36 @@
 Require Import Reflex.
 Require Import ReflexEcho.
+Import Spec.
 Require Import PolLang.
 Require Import ActionMatch.
 Require Import Tactics.
 
 Theorem recv_before : forall st tr m,
-  Reach _ _ COMPS _ _ _ INIT HANDLERS st -> ktr _ _ _ _ st = inhabits tr ->
-  ImmBefore PAYD
-            (KORecv PAYD None
+  Reach PAYD COMPT COMPTDEC COMPS KSTD IENVD INIT HANDLERS st ->
+  ktr _ _ _ _ st = inhabits tr ->
+  ImmBefore PAYD COMPT COMPS COMPTDEC
+            (KORecv PAYD COMPT COMPS None
                      (Some (Build_opt_msg PAYD
-                                           None (Some m, tt))))
-            (KOSend PAYD None
+                                          None (Some m, tt))))
+            (KOSend PAYD COMPT COMPS None
                      (Some (Build_opt_msg PAYD
-                                           None (Some m, tt))))
+                                          None (Some m, tt))))
             tr.
 Proof.
-  crush.
+  intros;
+  match goal with
+  | [ _ : ktr _ _ _ _ _ = inhabits ?tr, H : Reach _ _ _ _ _ _ _ _ _ |- _ ]
+      => generalize dependent tr; induction H;
+         (*Do not put simpl anywhere in here. It breaks destruct_unpack.*)
+         intros; destruct_unpack
+  end.
+match_immbefore.
+
 Qed.
 
 Theorem send_after : forall st tr m,
-  Reach _ _ COMPS _ _ _ INIT HANDLERS st -> ktr _ _ _ _ st = inhabits tr ->
-  ImmAfter PAYD
+  Reach st -> ktr _ _ _ _ st = inhabits tr ->
+  ImmAfter PAYD COMPT COMPS COMPTDEC
             (KOSend PAYD None
                      (Some (Build_opt_msg PAYD
                                            None (Some m, tt))))
